src/OeufProof.v
@@ -1,0 +1,48 @@
+Require Import Oeuf.
+Require Import CompilationUnit.
+Require Import HList.
+Require Import Untyped.
+
+Require Import compcert.lib.Coqlib.
+Require Import compcert.ia32.Asm.
+Require Import compcert.common.AST.
+Require Import compcert.common.Smallstep.
+Require Import compcert.common.Errors.
+Require Import compcert.common.Events.
+Require Import compcert.common.Globalenvs.
+
+
+Inductive correspond (exp : Untyped.expr) (st : Asm.state).
+
+Inductive simple_star {A : Type} (step : A -> A -> Prop) : A -> A -> Prop :=
+| star_nil :
+    forall st,
+      simple_star step st st
+| star_left :
+    forall st1 st2 st3,
+      step st1 st2 ->
+      simple_star step st2 st3 ->
+      simple_star step st1 st3.
+
+Theorem OeufUntypedCorrect :
+  forall l md asmprog,
+    transf_untyped_to_asm (l,md) = OK asmprog ->
+    forall expr expr',
+      In expr l ->
+      simple_star Untyped.step expr expr' ->
+      exists rs m rs' m',
+        Asm.initial_state asmprog (Asm.State rs m) /\
+        star Asm.step (Genv.globalenv asmprog) (State rs m) E0 (State rs' m') /\
+        correspond expr' (State rs' m').
+Proof.
+  induction 3; intros.
+  (* Here we need the "if we have an untyped expr, we get an Asm initial state" lemma *)
+  (* We also need that that initial state corresponds to the expression *)
+  admit.
+
+  (* Here we need the *)
+  admit.
+  
+  (* *)
+Admitted.
+
